veric/semax_loop.v
@@ -114,21 +114,19 @@ destruct H4 as [w1 [w2 [? [? ?]]]].
 specialize (H0 w0 H3).
 specialize (H1 w0 H3).
 unfold expr_true, expr_false, Cnot in *.
+
 pose proof (typecheck_expr_sound _ _ _ _ TC_ENV TC2) as HTCb; simpl in HTCb.
 unfold liftx, lift, eval_unop in HTCb; simpl in HTCb.
 destruct (bool_val (typeof b) (eval_expr b rho)) as [b'|] eqn: Hb; [|contradiction].
 assert (assert_safe Espec psi vx tx (Kseq (if b' then c else d) :: k)
   (construct_rho (filter_genv psi) vx tx) w0) as Hw0.
-{ admit. }
-eapply own.bupd_mono, bupd_tc_expr, Hw0; auto.
-
-
-intros r Hr ora jm Hge Hphi.
+{ unfold tc_expr in TC2; simpl in TC2.
+  rewrite denote_tc_assert_andp in TC2; destruct TC2.
+  destruct b'; [apply H0 | apply H1]; split; subst; auto; split; auto; do 3 eexists; eauto; split;
+    auto; split; auto; apply bool_val_strict; auto; eapply typecheck_expr_sound; eauto. }
+eapply own.bupd_mono, bupd_tc_expr, Hw0; eauto.
+intros r [Htc Hr] ora jm Hge Hphi.
 generalize (eval_expr_relate _ _ _ _ _ b jm HGG Hge (guard_environ_e1 _ _ _ TC)); intro.
-unfold tc_expr in TC2'.
-simpl in TC2'.
-rewrite denote_tc_assert_andp in TC2'.
-destruct TC2' as [TC2' TC2'a].
 apply wlog_safeN_gt0; intro.
 subst r.
 change (level (m_phi jm)) with (level jm) in H9.
@@ -139,23 +137,15 @@ clear H10.
 apply (@safe_step'_back2  _ _ _ _ _ _ _ _ psi ora _ jm
         (State vx tx (Kseq (if b' then c else d) :: k)) jm' _).
 split3.
+assert (TCS := typecheck_expr_sound _ _ (m_phi jm) _ (guard_environ_e1 _ _ _ TC) Htc).
+unfold tc_expr in Htc.
+simpl in Htc.
+rewrite denote_tc_assert_andp in Htc.
+clear TC2'; destruct Htc as [TC2' TC2'a].
 rewrite <- (age_jm_dry H9); econstructor; eauto.
-apply age1_resource_decay; auto.
-apply age_level; auto.
-change (level (m_phi jm)) with (level jm).
-replace (level jm - 1)%nat with (level jm' ) by (apply age_level in H10; omega).
-eapply @age_safe; try apply H10.
-rewrite <- Hge in *.
-
-
-assert (TCS := typecheck_expr_sound _ _ w0 _ (guard_environ_e1 _ _ _ TC) TC2').
- unfold tc_expr in TC2'.
- simpl in TC2'.
- rewrite denote_tc_assert_andp in TC2'.
- destruct TC2' as [TC2' TC2'a].
-assert (exists b': bool, Cop.bool_val (eval_expr b rho) (typeof b) (m_dry jm) = Some b'). {
-clear - TS TC H TC2 TC2' TC2'a TCS Hphi.
- simpl in TCS. unfold_lift in TCS.
+{ assert (exists b': bool, Cop.bool_val (eval_expr b rho) (typeof b) (m_dry jm) = Some b') as [].
+  { clear - TS TC H TC2 TC2' TC2'a TCS.
+    simpl in TCS. unfold_lift in TCS.
  unfold Cop.bool_val;
  destruct (eval_expr b rho) eqn:H15;
  simpl; destruct (typeof b) as [ | [| | | ] [| ]| | [ | ] |  | | | | ];
@@ -171,82 +161,16 @@ simpl in TC2'; destruct TC2'; subst; eauto;
  simpl; rewrite Hp.
 split; auto.
 }
-clear TCS.
-(* typechecking proof *)
-destruct H9 as [b' ?].
-apply wlog_safeN_gt0; intro.
-subst w0.
-change (level (m_phi jm)) with (level jm) in H10.
-revert H10; case_eq (level jm); intros.
-omegaContradiction.
-apply levelS_age1 in H10. destruct H10 as [jm' ?].
-clear H11.
-apply (@safe_step'_back2  _ _ _ _ _ _ _ _ psi ora _ jm
-        (State vx tx (Kseq (if b' then c else d) :: k)) jm' _).
-split3.
-rewrite <- (age_jm_dry H10); econstructor; eauto.
+  rewrite H10; symmetry; eapply f_equal, bool_val_Cop; eauto. }
 apply age1_resource_decay; auto.
-apply age_level; auto.
+split; [apply age_level; auto|].
+erewrite (age1_ghost_of _ _ (age_jm_phi H9)) by (symmetry; apply ghost_of_approx).
+repeat intro; auto.
 change (level (m_phi jm)) with (level jm).
-replace (level jm - 1)%nat with (level jm' ) by (apply age_level in H10; omega).
-eapply @age_safe; try apply H10.
+replace (level jm - 1)%nat with (level jm' ) by (apply age_level in H9; omega).
+eapply @age_safe; try apply H9.
 rewrite <- Hge in *.
-destruct b'.
-*
-eapply H0; auto.
-split; auto.
-split; auto.
-rewrite andp_comm.
-unfold lift1.
-unfold tc_expr in TC2.
- simpl in TC2.
- rewrite denote_tc_assert_andp in TC2.
- destruct TC2 as [TC2 TC2a].
-rewrite prop_true_andp.
-do 2 econstructor; split3; eauto.
-eapply typecheck_expr_sound in TC2a; eauto.
-clear - H9 TC2 TC2a.
-unfold typed_true, strict_bool_val.
- unfold Cop.bool_val;
- destruct (eval_expr b rho) eqn:H16;
- simpl; destruct (typeof b) as [ | [| | | ] [| ]| | [ | ] |  | | | | ];
-   try contradiction;
-    intuition; simpl in *; try rewrite TCS; eauto;
-try (rewrite denote_tc_assert_andp in TC2; destruct TC2 as [TC2'' TC2]);
- try (rewrite binop_lemmas2.denote_tc_assert_test_eq' in  TC2;
- simpl in TC2; unfold_lift in TC2; rewrite H16 in TC2);
- destruct Archi.ptr64 eqn:Hp; try contradiction.
-simpl in TC2; rewrite Hp in TC2; simpl in TC2; destruct TC2; subst; eauto.
-*
-eapply H1; auto.
-split; auto.
-split; auto.
-unfold lift1.
-rewrite andp_comm; rewrite prop_true_andp.
-do 2 econstructor; split3; eauto.
-unfold tc_expr in TC2.
- simpl in TC2.
- rewrite denote_tc_assert_andp in TC2.
- destruct TC2 as [TC2 TC2a].
-eapply typecheck_expr_sound in TC2a; eauto.
-clear - H9 TC2 TC2a.
-unfold typed_true, strict_bool_val.
- unfold Cop.bool_val;
- destruct (eval_expr b rho) eqn:H16;
- simpl; destruct (typeof b) as [ | [| | | ] [| ]| | [ | ] |  | | | | ];
-   try contradiction;
-    intuition; simpl in *; try rewrite TCS; eauto;
-try (rewrite denote_tc_assert_andp in TC2; destruct TC2 as [TC2'' TC2]);
- try (rewrite binop_lemmas2.denote_tc_assert_test_eq' in  TC2;
- simpl in TC2; unfold_lift in TC2; rewrite H16 in TC2);
- destruct Archi.ptr64 eqn:Hp; try contradiction.
-simpl in TC2; rewrite Hp in TC2; simpl in TC2; destruct TC2; subst; eauto.
-unfold Cop.bool_val in H9.
-unfold typed_false.
-unfold classify_bool in H9.
-simpl in H9.
-rewrite Hp in H9.
-if_tac in H9; inv H9.
+apply Hr; auto.
 Qed.
 (*
 Lemma seq_assoc1:
@@ -614,73 +538,36 @@ Proof.
   generalize (pred_nec_hereditary _ _ _ NEC2 H3); intro H3'.
   remember (construct_rho (filter_genv psi) vx tx) as rho.
   pose proof I.
-  intros ora jm RE H11.
-  pose (H10:=True).
-  replace (level a') with (S (level a2))
-    by (apply age_level in LEVa2;  rewrite LEVa2; apply minus_n_O).
-  subst a'.
-  destruct (can_age1_juicy_mem _ _ LEVa2) as [jm' LEVa2'].
-  unfold age in LEVa2.
-  assert (a2 = m_phi jm').
-  Focus 1. {
-    generalize (age_jm_phi LEVa2'); unfold age; change R.rmap with rmap.
-    change R.ag_rmap with ag_rmap; rewrite LEVa2.
-    intro Hx; inv Hx; auto.
-  } Unfocus.
-  subst a2.
-  clear LEVa2; rename LEVa2' into LEVa2.
-  apply safe_corestep_backward
-   with (State vx tx (Kseq body :: Kseq Scontinue :: Kloop1 body incr :: k))
-          jm'.
-  Focus 1. {
-    split3.
-    + rewrite (age_jm_dry LEVa2); econstructor.
-    + apply age1_resource_decay; auto.
-    + apply age_level; auto.
-  } Unfocus.
   eapply semax_extensionality_Delta in H; try apply TS; auto.
   eapply semax_extensionality_Delta in H0; try apply TS; auto.
   clear Delta TS.
-  assert (w >= level (m_phi jm)).
-  Focus 1. {
-    apply necR_nat in H5. apply nec_nat in H5.
-    change R.rmap with rmap in *; omega.
-  } Unfocus.
-  clear y H5 H4. rename H11 into H5. pose (H4:=True).
   generalize H; rewrite semax_unfold; intros H'.
-  change ((believe Espec Delta' psi Delta') (level jm')) in Prog_OK2.
-  specialize (H' psi Delta' (level jm') (tycontext_sub_refl _) HGG Prog_OK2 (Kseq Scontinue :: Kloop1 body incr :: k) F CLO_body).
+(*  change ((believe Espec Delta' psi Delta') (level jm')) in Prog_OK2.*)
+  specialize (H' psi Delta' (level a2) (tycontext_sub_refl _) HGG Prog_OK2 (Kseq Scontinue :: Kloop1 body incr :: k) F CLO_body).
   spec H'.
-  Focus 2. {
-    apply (H' tx vx _ (le_refl _) (m_phi jm') (necR_refl _)); try solve[subst; auto].
-    apply pred_hereditary with (m_phi jm); auto.
-    + apply age_jm_phi; auto.
-    + subst.
-      split; auto.
-      split; auto.
-  } Unfocus.
+  { 
   intros ek vl.
   destruct ek.
   + simpl exit_cont.
     rewrite semax_unfold in H0.
-    specialize (H0 psi _ (level jm') (tycontext_sub_refl _)  HGG Prog_OK2 (Kloop2 body incr :: k) F CLO_incr).
+    specialize (H0 psi _ (level a2) (tycontext_sub_refl _)  HGG Prog_OK2 (Kloop2 body incr :: k) F CLO_incr).
     spec H0.
     Focus 1. {
       intros ek2 vl2 tx2 vx2.
       destruct ek2; simpl exit_tycon in *.
       + unfold exit_cont.
         apply (assert_safe_adj' Espec) with (k:=Kseq (Sloop body incr) :: k); auto.
-        - repeat intro. eapply convergent_controls_safe; try apply H12; simpl; auto.
-          intros q' m' [? [? ?]]; split3; auto. inv H13; econstructor; eauto.
+        - repeat intro. eapply convergent_controls_safe; try apply H11; simpl; auto.
+          intros q' m' [? [? ?]]; split3; auto. inv H12; econstructor; eauto.
         - eapply subp_trans'; [ |  eapply (H1 _ LT Prog_OK2 H3' tx2 vx2)].
           apply derives_subp.
           rewrite funassert_update_tycon.
           apply andp_derives; auto.
           apply andp_derives; auto.
           * intros ? [? ?]; split; auto.
-            hnf in H11|-*.
+            hnf in H10|-*.
             eapply typecheck_environ_update; eauto.
-            simpl in H12|-*. rewrite ret_type_update_tycon in H12; auto.
+            simpl in H11|-*. rewrite ret_type_update_tycon in H11; auto.
           * simpl exit_cont.
             rewrite proj_frame_ret_assert. simpl proj_ret_assert. simpl seplog.sepcon.
             normalize.
@@ -713,7 +600,7 @@ Proof.
       intros ? [? ?]; split.
       * hnf in H11|-*.
         eapply typecheck_environ_update; eauto.
-      * simpl in H12|-*; rewrite ret_type_update_tycon in H12; auto.
+      * simpl in H11|-*; rewrite ret_type_update_tycon in H11; auto.
     - simpl exit_cont.
       simpl exit_tycon.
       rewrite sepcon_comm. destruct POST; simpl proj_ret_assert. normalize.
@@ -744,7 +631,7 @@ Proof.
     apply (assert_safe_adj' Espec) with (k:=Kseq (Sloop body incr) :: k); auto.
     - intros ? ? ? ? ? ? ?.
       eapply convergent_controls_safe; simpl; eauto.
-      intros q' m' [? [? ?]]; split3; auto. inv H12; econstructor; eauto.
+      intros q' m' [? [? ?]]; split3; auto. inv H11; econstructor; eauto.
     - eapply subp_trans'; [ | eapply H1; eauto].
       apply derives_subp.
       rewrite funassert_exit_tycon;
@@ -754,7 +641,7 @@ Proof.
         intros ? [? ?]; split.
         hnf in H11|-*.
         eapply typecheck_environ_update; eauto.
-        simpl in H12|-*; rewrite ret_type_update_tycon in H12; auto.
+        simpl in H11|-*; rewrite ret_type_update_tycon in H11; auto.
       * unfold exit_cont, loop2_ret_assert; normalize.
         specialize (H3' EK_return vl2 tx2 vx2). simpl exit_tycon in H3'.
         intros tx4 vx4.
@@ -776,7 +663,40 @@ Proof.
     eapply subp_trans'; [ | eapply (H3' EK_return) ; eauto].
      simpl exit_tycon.
     simpl proj_ret_assert. destruct POST; simpl tycontext.RA_return.
-    apply subp_refl'.
+    apply subp_refl'. }
+  specialize (H' tx vx _ (le_refl _) _ (necR_refl _)); spec H'.
+  { apply pred_hereditary with a'; auto.
+    subst; split; auto; split; auto. }
+  simpl in H'.
+  destruct (H' (core (ghost_of a2))) as (b & ? & m' & Hl & Hr & ? & Hsafe); subst.
+  { rewrite <- ghost_of_approx at 1; eexists; apply ghost_fmap_join, join_comm, core_unit. }
+  apply own.bupd_intro.
+  intros ora jm RE ?; subst.
+  destruct (can_age1_juicy_mem _ _ LEVa2) as [jm2 LEVa2'].
+  unfold age in LEVa2.
+  assert (a2 = m_phi jm2).
+  Focus 1. {
+    generalize (age_jm_phi LEVa2'); unfold age; change R.rmap with rmap.
+    change R.ag_rmap with ag_rmap; rewrite LEVa2.
+    intro Hx; inv Hx; auto.
+  } Unfocus.
+  subst a2.
+  destruct (juicy_mem_resource _ _ Hr) as (jm' & ? & Hdry); subst.
+  rewrite (age_level _ _ LEVa2).
+  apply safe_corestep_backward
+   with (State vx tx (Kseq body :: Kseq Scontinue :: Kloop1 body incr :: k))
+          jm'.
+  Focus 1. {
+    split3.
+    + rewrite (age_jm_dry LEVa2'), Hdry; econstructor.
+    + destruct (age1_resource_decay _ _ LEVa2') as [? Hdecay].
+      split; [rewrite Hl; auto|].
+      intro l; rewrite Hl, Hr; auto.
+    + split; [unfold level; simpl; rewrite Hl; apply age_level; auto|].
+      
+  } Unfocus.
+  
+  specialize (H' _ (core_unit _
 Qed.
 
 Lemma semax_break {CS: compspecs}:
